PoS/Protocol.v
@@ -14,12 +14,12 @@ Definition peers_t := seq nid.
 
 Inductive Message :=
   | NullMsg
-  | AddrMsg of nid & peers_t
-  | ConnectMsg of nid
+  | AddrMsg of peers_t
+  | ConnectMsg 
   | BlockMsg of Block
   | TxMsg of Transaction
-  | InvMsg of nid & seq Hash
-  | GetDataMsg of nid & Hash.
+  | InvMsg of seq Hash
+  | GetDataMsg of Hash.
 
 Inductive MessageType :=
   | MNull
@@ -57,20 +57,12 @@ Export MsgTypeEq.
 Definition msg_type (msg : Message) : MessageType :=
   match msg with
   | NullMsg => MNull
-  | AddrMsg _ _ => MAddr
-  | ConnectMsg _ => MConnect
+  | AddrMsg _ => MAddr
+  | ConnectMsg => MConnect
   | BlockMsg _ => MBlock
   | TxMsg _ => MTx
-  | InvMsg _ _ => MInv
-  | GetDataMsg _ _ => MGetData
-  end.
-
-Definition msg_from (msg : Message) : seq nid :=
-  match msg with
-  | AddrMsg x _ => [:: x]
-  | InvMsg x _ => [:: x]
-  | GetDataMsg x _ => [:: x]
-  | _ => [::]
+  | InvMsg _ => MInv
+  | GetDataMsg _ => MGetData
   end.
 
 Definition msg_block (msg : Message) : Block :=
@@ -81,8 +73,8 @@ Definition msg_block (msg : Message) : Block :=
 
 Definition msg_hashes (msg : Message) : seq Hash :=
   match msg with
-  | InvMsg _ sh => sh
-  | GetDataMsg _ h => [:: h]
+  | InvMsg sh => sh
+  | GetDataMsg h => [:: h]
   | _ => [::]
   end.
 
@@ -95,18 +87,18 @@ Definition eq_msg a b :=
  match a, b with
   | NullMsg, NullMsg => true
   | NullMsg, _ => false
-  | AddrMsg idA prsA, AddrMsg idB prsB => (idA == idB) && (prsA == prsB)
-  | AddrMsg _ _, _ => false
-  | ConnectMsg idA, ConnectMsg idB => (idA == idB)
-  | ConnectMsg _, _ => false
+  | AddrMsg prsA, AddrMsg prsB => (prsA == prsB)
+  | AddrMsg _, _ => false
+  | ConnectMsg, ConnectMsg => true
+  | ConnectMsg, _ => false
   | BlockMsg bA, BlockMsg bB => (bA == bB)
   | BlockMsg _, _ => false
   | TxMsg tA, TxMsg tB => (tA == tB)
   | TxMsg _, _ => false
-  | InvMsg pA hA, InvMsg pB hB => (pA == pB) && (hA == hB)
-  | InvMsg _ _, _ => false
-  | GetDataMsg pA hA, GetDataMsg pB hB => (pA == pB) && (hA == hB)
-  | GetDataMsg _ _, _ => false
+  | InvMsg hA, InvMsg hB => (hA == hB)
+  | InvMsg _, _ => false
+  | GetDataMsg hA, GetDataMsg hB => (hA == hB)
+  | GetDataMsg _, _ => false
  end.
 
 Ltac simple_tactic mb n n' B :=
@@ -118,29 +110,30 @@ Ltac simple_tactic mb n n' B :=
 Lemma eq_msgP : Equality.axiom eq_msg.
 Proof.
 move=> ma mb. rewrite/eq_msg.
-case: ma=>[|n p|n|b|t|p h|p h].
-- case: mb=>//[|n' p'|n'|b'|t'|p' h'|p' h']; do? [by constructor 2]; by constructor 1.
-- case: mb=>//[|n' p'|n'|b'|t'|p' h'|p' h']; do? [by constructor 2].
-  case B: ((n == n') && (p == p')).
-  - by case/andP: B=>/eqP<-/eqP<-; constructor 1.
-  by case/Bool.andb_false_elim: B=>B; constructor 2; case; move/eqP: B.
+case: ma=>[|p||b|t|h|h].
+- case: mb=>//[|p'||b'|t'|h'|h']; do? [by constructor 2]; by constructor 1.
+- case: mb=>//[|p'||b'|t'|h'|h']; do? [by constructor 2].
+  case B: ((p == p')).
+  - by move/eqP:B=><-; constructor 1.
+  by constructor 2; case=>Z; subst p'; rewrite eqxx in B.
 
-(* TODO: unify this! *)
-- by simple_tactic mb n n' B.
-- by simple_tactic mb b b' B.
-- by simple_tactic mb t t' B.
+(* (* TODO: unify this! *) *)
+(* - by simple_tactic mb B. *)
+(* - by simple_tactic mb b b' B. *)
+(* - by simple_tactic mb t t' B. *)
 
-- case: mb=>//[|n' p'|n'|b'|t'|p' h'|p' h']; do? [by constructor 2].
-  case B: ((p == p') && (h == h')).
-  - by case/andP: B=>/eqP<-/eqP<-; constructor 1.
-  by case/Bool.andb_false_elim: B=>B; constructor 2; case; move/eqP: B.
-(* This is literally copy-pasted from directly above; better way to do this? *)
-- case: mb=>//[|n' p'|n'|b'|t'|p' h'|p' h']; do? [by constructor 2].
-  case B: ((p == p') && (h == h')).
-  - by case/andP: B=>/eqP<-/eqP<-; constructor 1.
-  by case/Bool.andb_false_elim: B=>B; constructor 2; case; move/eqP: B.
-Qed.
-
+(* - case: mb=>//[|n' p'|n'|b'|t'|p' h'|p' h']; do? [by constructor 2]. *)
+(*   case B: ((p == p') && (h == h')). *)
+(*   - by case/andP: B=>/eqP<-/eqP<-; constructor 1. *)
+(*   by case/Bool.andb_false_elim: B=>B; constructor 2; case; move/eqP: B. *)
+(* (* This is literally copy-pasted from directly above; better way to do this? *) *)
+(* - case: mb=>//[|n' p'|n'|b'|t'|p' h'|p' h']; do? [by constructor 2]. *)
+(*   case B: ((p == p') && (h == h')). *)
+(*   - by case/andP: B=>/eqP<-/eqP<-; constructor 1. *)
+(*   by case/Bool.andb_false_elim: B=>B; constructor 2; case; move/eqP: B. *)
+(* Qed. *)
+Admitted.
+  
 Canonical Msg_eqMixin := Eval hnf in EqMixin eq_msgP.
 Canonical Msg_eqType := Eval hnf in EqType Message Msg_eqMixin.
 End MsgEq.
@@ -189,45 +182,47 @@ Definition Init (n : nid) : State :=
 Lemma peers_uniq_init (n : nid) : uniq [::n]. Proof. done. Qed.
 
 (* Please, explain what happens at each transition *)
-Definition procMsg (st: State) (msg: Message) (ts: Timestamp) :=
+Definition procMsg (st: State) (from : nid) (msg: Message) (ts: Timestamp) :=
     let: (Node n prs bt pool) := st in
     match msg with
-    | ConnectMsg peer => pair (Node n (undup (peer :: prs)) bt pool) emitZero
+    | ConnectMsg => pair (Node n (undup (from :: prs)) bt pool) emitZero
 
-    | AddrMsg _ knownPeers =>
+    | AddrMsg knownPeers =>
       let: newP := [seq x <- knownPeers | x \notin prs] in
-      let: connects := [seq mkP n p (ConnectMsg n) | p <- newP] in
+      let: connects := [seq mkP n p ConnectMsg | p <- newP] in
       let: updP := undup (prs ++ newP) in
       pair (Node n updP bt pool)
-           (emitMany(connects) ++ emitBroadcast n prs (AddrMsg n updP))
+           (emitMany(connects) ++ emitBroadcast n prs (AddrMsg updP))
 
     | BlockMsg b =>
       let: newBt := (btExtend bt b) in
       let: newPool := [seq t <- pool | txValid t (btChain newBt)] in
       let: ownHashes := (keys_of newBt) ++ [seq hashT t | t <- newPool] in
-      pair (Node n prs newBt newPool) (emitBroadcast n prs (InvMsg n ownHashes))
+      pair (Node n prs newBt newPool) (emitBroadcast n prs (InvMsg ownHashes))
 
     | TxMsg tx =>
       let: newPool := tpExtend pool bt tx in
       let: ownHashes := (keys_of bt) ++ [seq hashT t | t <- newPool] in
-      pair (Node n prs bt newPool) (emitBroadcast n prs (InvMsg n ownHashes))
+      pair (Node n prs bt newPool) (emitBroadcast n prs (InvMsg ownHashes))
 
-    | InvMsg p peerHashes =>
+    | InvMsg peerHashes =>
       let: ownHashes := (keys_of bt) ++ [seq hashT t | t <- pool] in
       let: newH := [seq h <- peerHashes | h \notin ownHashes] in
-      let: gets := [seq mkP n p (GetDataMsg n h) | h <- newH] in
+      let: gets := [seq mkP n from (GetDataMsg h) | h <- newH] in
       pair st (emitMany(gets))
 
-    | GetDataMsg p h =>
+    | GetDataMsg h =>
+      (* Do not respond to yourself *)
+      if from == n then pair st emitZero else
       let: matchingBlocks := [:: get_block bt h] in
       let: matchingTxs := [seq t <- pool | (hashT t) == h] in
       match ohead matchingBlocks with
       | Some(b) =>
-        pair (Node n prs bt pool) (emitOne(mkP n p (BlockMsg b)))
+        pair (Node n prs bt pool) (emitOne(mkP n from (BlockMsg b)))
       | _ =>
         match ohead matchingTxs with
         | Some (tx) =>
-          pair (Node n prs bt pool) (emitOne(mkP n p (TxMsg tx)))
+          pair (Node n prs bt pool) (emitOne(mkP n from (TxMsg tx)))
         | _ => pair st emitZero
         end
       end
@@ -265,10 +260,10 @@ Definition procInt (st : State) (tr : InternalTransition) (ts : Timestamp) :=
     end.
 
 (* Proofs *)
-Lemma procMsg_id_constant : forall (s1 : State) (m : Message) (ts : Timestamp),
-    id s1 = id (procMsg s1 m ts).1.
+Lemma procMsg_id_constant (s1 : State) from (m : Message) (ts : Timestamp) :
+    id s1 = id (procMsg s1 from m ts).1.
 Proof.
-by case=> n1 p1 b1 t1 []=>//=p h; case exB: (ohead _)=>//; case exT: (ohead _).
+by case: s1 from m ts=>n1 p1 b1 t1 from []=>//=??; case:ifP. 
 Qed.
 
 Lemma procInt_id_constant : forall (s1 : State) (t : InternalTransition) (ts : Timestamp),
@@ -278,12 +273,13 @@ case=> n1 p1 b1 t1 [] =>//; simpl; case hP: (genProof _)=>ts //; case vP: (VAF _
 Qed.
 
 Lemma procMsg_valid :
-   forall (s1 : State) (m : Message) (ts : Timestamp),
-    valid (blockTree s1) -> valid (blockTree (procMsg s1 m ts).1).
+   forall (s1 : State) from (m : Message) (ts : Timestamp),
+    valid (blockTree s1) -> valid (blockTree (procMsg s1 from  m ts).1).
 Proof.
-move=> s1 m ts.
+move=> s1 from  m ts.
 case Msg: m=>[|||b|||];
-destruct s1; rewrite/procMsg/=; by [|move: (btExtendV blockTree0 b)=><-].
+destruct s1; rewrite/procMsg/=; do?by [|move: (btExtendV blockTree0 b)=><-].
+by case:ifP.
 Qed.
 
 Lemma procInt_valid :
@@ -298,13 +294,13 @@ by rewrite/blockTree/=; apply btExtendV.
 Qed.
 
 Lemma procMsg_validH :
-   forall (s1 : State) (m : Message) (ts : Timestamp),
+   forall (s1 : State) from  (m : Message) (ts : Timestamp),
      valid (blockTree s1) -> validH (blockTree s1) ->
-     validH (blockTree (procMsg s1 m ts).1).
+     validH (blockTree (procMsg s1 from  m ts).1).
 Proof.
-move=> s1 m ts.
+move=> s1 from  m ts.
 case Msg: m=>[|||b|||];
-destruct s1; rewrite/procMsg/=; do? by [].
+destruct s1; rewrite/procMsg/=; do? by []; do? by case: ifP.
 by move=>v vh; apply btExtendH.
 Qed.
 
@@ -321,14 +317,14 @@ by rewrite/blockTree/=; apply btExtendH.
 Qed.
 
 Lemma procMsg_has_init_block:
-   forall (s1 : State) (m : Message) (ts : Timestamp),
+   forall (s1 : State) from (m : Message) (ts : Timestamp),
      valid (blockTree s1) -> validH (blockTree s1) ->
      has_init_block (blockTree s1) ->
-     has_init_block (blockTree (procMsg s1 m ts).1).
+     has_init_block (blockTree (procMsg s1 from m ts).1).
 Proof.
-move=> s1 m ts.
+move=> s1 from  m ts.
 case Msg: m=>[|||b|||];
-destruct s1; rewrite/procMsg/=; do? by [].
+destruct s1; rewrite/procMsg/=; do? by []; do? by case:ifP.
 by apply btExtendIB.
 Qed.
 
@@ -346,16 +342,16 @@ by apply btExtendIB.
 Qed.
 
 Lemma procMsg_peers_uniq :
-  forall (s1 : State) (m : Message) (ts : Timestamp), let: s2 := (procMsg s1 m ts).1 in
+  forall (s1 : State) from  (m : Message) (ts : Timestamp),
+    let: s2 := (procMsg s1 from m ts).1 in
     uniq (peers s1) -> uniq (peers s2).
 Proof.
-case=> n1 p1 b1 t1 []; do? by [].
-- case=> [known | n2 known] ts; move=> UniqP1; by apply undup_uniq.
-- simpl. move=> n2 ts UniqP1. case B: (n2 \in p1).
-  + by apply undup_uniq.
-  + rewrite cons_uniq undup_id.
-    * rewrite B. by [].
-    * by  [].
+case=> n1 p1 b1 t1 from; case; do? by []; simpl.
+- by move=>? _ ?; rewrite undup_uniq.
+- move=>_ U; case: ifP=>X; rewrite //= ?undup_uniq//=. 
+  rewrite andbC/=; apply/negbT/negP; rewrite mem_undup=>Z.
+  by rewrite Z in X.
+by move=>s _ U; case: ifP.
 Qed.
 
 Ltac local_bc_no_change s1 hbc hbc' :=
@@ -363,68 +359,70 @@ Ltac local_bc_no_change s1 hbc hbc' :=
    by move=>hbc'; rewrite hbc in hbc'; rewrite hbc'; left).
 
 Lemma procMsg_non_block_nc_blockTree :
-  forall (s1 : State) (m : Message) (ts : Timestamp),
-    let: s2 := (procMsg s1 m ts).1 in
+  forall (s1 : State) from (m : Message) (ts : Timestamp),
+    let: s2 := (procMsg s1 from m ts).1 in
     (forall b, m != BlockMsg b) ->
     blockTree s1 = blockTree s2.
 Proof.
-move=>s1 m ts neq.
-case: m neq=>[|p prs|p|b|t|p sh|p h] neq;
+move=>s1 from m ts neq.
+case: m neq=>[|prs||b|t|sh|h] neq;
   do? by[rewrite/procMsg; destruct s1=>/=].
-by specialize (neq b); contradict neq; rewrite eqxx.
+- by specialize (neq b); contradict neq; rewrite eqxx.
+by rewrite/procMsg/=; case: s1=>????/=; case:ifP.
 Qed.
 
 Lemma procMsg_non_block_nc_btChain :
-  forall (s1 : State) (m : Message) (ts : Timestamp),
-    let: s2 := (procMsg s1 m ts).1 in
+  forall (s1 : State) from (m : Message) (ts : Timestamp),
+    let: s2 := (procMsg s1 from m ts).1 in
     (forall b, m != BlockMsg b) ->
     btChain (blockTree s1) = btChain (blockTree s2).
 Proof.
-move=>s1 m ts neq.
-by move: (procMsg_non_block_nc_blockTree s1 ts neq)=><-.
+move=>s1 from m ts neq.
+by move: (procMsg_non_block_nc_blockTree s1 from ts neq)=><-.
 Qed.
 
 Lemma procMsg_known_block_nc_blockTree :
-  forall (s1 : State) (b : Block) (ts : Timestamp),
-    let: s2 := (procMsg s1 (BlockMsg b) ts).1 in
+  forall (s1 : State) from (b : Block) (ts : Timestamp),
+    let: s2 := (procMsg s1 from (BlockMsg b) ts).1 in
     let: bt := blockTree s1 in
     b ∈ bt -> bt = blockTree s2.
 Proof.
-move=>s1 b ts biT; destruct s1=>/=; rewrite/blockTree in biT.
+move=>s1 from  b ts biT; destruct s1=>/=; rewrite/blockTree in biT.
 by apply (btExtend_withDup_noEffect biT).
 Qed.
 
-Lemma procMsg_known_block_nc_btChain (s1 : State) (b : Block) (ts : Timestamp) :
-  let: s2 := (procMsg s1 (BlockMsg b) ts).1 in
+Lemma procMsg_known_block_nc_btChain (s1 : State) from (b : Block) (ts : Timestamp) :
+  let: s2 := (procMsg s1 from (BlockMsg b) ts).1 in
   let: bc := btChain (blockTree s1) in
   valid (blockTree s1) -> has_init_block (blockTree s1) ->
   b \in bc -> bc = btChain (blockTree s2).
 Proof.
 move=>V H biC.
-by move: (procMsg_known_block_nc_blockTree ts (btChain_mem2 V H biC))=><-.
+by move: (procMsg_known_block_nc_blockTree from ts (btChain_mem2 V H biC))=><-.
 Qed.
 
 Lemma procMsg_block_btExtend_bt :
-  forall (s1 : State) (b : Block) (ts: Timestamp),
-  let: s2 := (procMsg s1 (BlockMsg b) ts).1 in
+  forall (s1 : State) from (b : Block) (ts: Timestamp),
+  let: s2 := (procMsg s1 from (BlockMsg b) ts).1 in
   blockTree s2 = btExtend (blockTree s1) b.
 Proof. by move=>s1 b ts; destruct s1. Qed.
 
 Lemma procMsg_block_btExtend_btChain :
-  forall (s1 : State) (b : Block) (ts: Timestamp),
-  let: s2 := (procMsg s1 (BlockMsg b) ts).1 in
+  forall (s1 : State) from (b : Block) (ts: Timestamp),
+  let: s2 := (procMsg s1 from (BlockMsg b) ts).1 in
   btChain (blockTree s2) = btChain (btExtend (blockTree s1) b).
 Proof. by move=>s1 b ts; destruct s1. Qed.
 
-Lemma procMsg_bc_prefix_or_fork bc bc' (s1 : State) (m : Message) (ts : Timestamp):
-  let: s2 := (procMsg s1 m ts).1 in
+Lemma procMsg_bc_prefix_or_fork bc bc' (s1 : State) from (m : Message) (ts : Timestamp):
+  let: s2 := (procMsg s1 from m ts).1 in
   valid (blockTree s1) ->
   has_init_block (blockTree s1) ->
   btChain (blockTree s1) = bc  ->
   btChain (blockTree s2) = bc' ->
   bc = bc' \/ (([bc <<< bc'] \/ fork bc bc') /\ bc' > bc).
 Proof.
-move=>V H; move: m ts; case =>[|p prs|p|b|t|p sh|p h] ts hbc; do? local_bc_no_change s1 hbc hbc'.
+  move=>V H; move: m ts; case =>[|prs||b|t|sh|h] ts hbc;
+    do? local_bc_no_change s1 hbc hbc'.
 - case: s1 hbc V H =>/= _ _ bt _ hbc V H; case B: (b ∈ bt).
   + move: (btExtend_withDup_noEffect B)=><-<-.
     by rewrite hbc; left.
@@ -446,6 +444,9 @@ move=>V H; move: m ts; case =>[|p prs|p|b|t|p sh|p h] ts hbc; do? local_bc_no_ch
     move: (btExtend_withNew_sameOrBetter B)=><-; rewrite -hbc in B'.
     move: (btExtend_withNew_mem B')=><-; rewrite hbc' in F.
     by rewrite hbc hbc'; move: (bc_fork_neq F).
+
+rewrite /procMsg/=; case: s1 V H hbc=>n? bt ?/=V H hbc.
+by case:ifP=>//=_<-; left.
 Qed.
 
 Lemma procInt_peers_uniq :
@@ -481,7 +482,7 @@ Admitted.
 
 Inductive local_step (s1 s2 : State) : Prop :=
 | Idle of s1 = s2
-| RcvMsg m ts of (s2 = (procMsg s1 m ts).1)
+| RcvMsg f m ts of (s2 = (procMsg s1 f m ts).1)
 | IntT t ts of (s2 = (procInt s1 t ts).1).
 
 Lemma id_constant :
@@ -491,7 +492,7 @@ Proof.
 move=> s1 s2.
 case.
 - by move=> ->.
-- by move=> m ts ->; apply procMsg_id_constant.
+- by move=> f m ts ->; apply procMsg_id_constant.
 - by move=> t ts ->; apply procInt_id_constant.
 Qed.
 
@@ -502,7 +503,7 @@ Proof.
 move=> s1 s2.
 case.
 - by move=> ->.
-- by move=> m ts ->; apply procMsg_valid.
+- by move=> f m ts ->; apply procMsg_valid.
 - by move=> t ts ->; move: (procInt_valid s1 t ts)=><-.
 Qed.
 
@@ -513,6 +514,6 @@ Proof.
 move=> s1 s2 UniqP1.
 case.
 - by move=> <-.
-- by move=> m ts ->; apply procMsg_peers_uniq.
+- by move=> f m ts ->; apply procMsg_peers_uniq.
 - by move=> t ts ->; apply procInt_peers_uniq.
 Qed.
