PoS/InvCliqueTopology.v
@@ -19,7 +19,6 @@ blocks towars it "in flight" are received and used to extend the local
 block tree.  *)
 (*******************************************************************)
 
-
 Definition GSyncing_clique w :=
   exists (bc : Blockchain) (n : nid),
   [/\ holds n w (has_chain bc),
@@ -54,21 +53,51 @@ Qed.
 
 Ltac NBlockMsg_dest_bt q st p b Msg H :=
   (have: (forall b, msg p != BlockMsg b) by move=>b; rewrite Msg)=>H;
-  move: (procMsg_non_block_nc_blockTree st (ts q) H).
+  move: (procMsg_non_block_nc_blockTree st (src p) (ts q) H).
 
 Ltac NBlockMsg_dest_btChain q st p b Msg P H :=
   (have: (forall b, msg p != BlockMsg b) by move=>b; rewrite Msg)=>H;
-  move: (procMsg_non_block_nc_btChain st (ts q) H);
+  move: (procMsg_non_block_nc_btChain st (src p) (ts q) H);
   rewrite/has_chain Msg P /==><-.
 
-Ltac BlockMsg_dest q st b iF P Msg :=
-  rewrite [procMsg _ _ _] surjective_pairing in P; case: P=><- _;
-  rewrite/has_chain (procMsg_block_btExtend_btChain st b (ts q));
+Ltac BlockMsg_dest q st from b iF P Msg :=
+  rewrite [procMsg _ _ _ _] surjective_pairing in P; case: P=><- _;
+  rewrite/has_chain (procMsg_block_btExtend_btChain st from b (ts q));
   move: (b_in_blocksFor iF Msg)=>iB.
 
 Ltac simplw w :=
 have: ((let (_, inFlightMsgs, _) := w in inFlightMsgs) = inFlightMsgs w) by [];
 have: ((let (localState, _, _) := w in localState) = localState w) by [].
+
+(*********************************************************)
+(*                  Auxiliary Lemmas                     *)
+(*********************************************************)
+
+(* (* procMsg emits no block messages *) *)
+(* Lemma procMsg_no_blocks st p q stPm ms n' : *)
+(*   procMsg st (src p) (msg p) (ts q) = (stPm, ms) -> *)
+(*   all (pred1 GenesisBlock) [seq msg_block (msg p0) | p0 <- ms & dst p0 == n']. *)
+(* Proof. *)
+(* rewrite [procMsg _ _ _ _]surjective_pairing; case=>_{stPm}<-{ms}. *)
+(* case (msg p); rewrite /procMsg/=; case: st=>id ps bt tp/=. *)
+(* - by case: ifP=>//_; apply/allP=>m; rewrite inE=>/eqP->/=; rewrite eqxx.  *)
+(* - move=>pt; apply/allP=>m; rewrite !inE. *)
+(*   move/mapP=>[z]; rewrite mem_filter/emitMany/emitBroadcast=>/andP[_]. *)
+(*   by rewrite mem_cat=>/orP[]/=; move/mapP=>[y]_->->/=; rewrite eqxx. *)
+(* - by apply/allP=>b; case: ifP=>//_; rewrite inE=>/eqP->/=;rewrite eqxx. *)
+(* - move=>c; apply/allP=>b/mapP[z]; rewrite mem_filter=>/andP[_]. *)
+(*   by move/mapP=>[n]_->->/=; rewrite eqxx. *)
+(* - move=>t; apply/allP=>z/mapP[y]; rewrite mem_filter=>/andP[_]. *)
+(*   by move/mapP=>[n]_->->/=; rewrite eqxx. *)
+(* - move=>l; apply/allP=>z/mapP[y]; rewrite mem_filter=>/andP[_]. *)
+(*   by move/mapP=>[m]_->->/=; rewrite eqxx. *)
+(* move=>t; apply/allP=>z/mapP[y]; case:ifP=>X//=. *)
+(* - by case:ifP=>//_; rewrite inE=>/eqP->->. *)
+(* case: ifP=>//=/eqP Z; rewrite inE=>/eqP->->/=. *)
+(* (* Ok, this is not true, as p might be a GetData request :( *) *)
+(* Admitted.   *)
+  
+(*********************************************************)
 
 (* TODO: Now the inductive version. *)
 Lemma clique_inv_step w w' q :
@@ -82,7 +111,7 @@ case: Iw=>_ [GStabW|GSyncW].
 - by case GStabW=>noPackets; contradict iF; rewrite noPackets.
 - case: GSyncW=>can_bc [can_n] [] HHold HGt HCliq (*[HCon1 HCon2]*) HExt.
   move=>P; assert (P' := P).
-  move: P; case P: (procMsg _ _ _)=>[stPm ms]; move=>->; right.
+  move: P; case P: (procMsg _ _ _ _)=>[stPm ms]; move=>->; right.
   (* The canonical chain is guaranteed to remain the same for any Msg *)
   exists can_bc, can_n; split.
 
@@ -91,7 +120,7 @@ case: Iw=>_ [GStabW|GSyncW].
     move/eqP=>Eq [Eq']; subst can_n stPm.
     case Msg: (msg p)=>[|||b|||]; rewrite Msg in P;
     do? by [NBlockMsg_dest_btChain q st p b Msg P H; move: (HHold _ F)].
-    by BlockMsg_dest q st b iF P Msg; move: (c3 (dst p) _ F)=>V;
+    by BlockMsg_dest q st (src p) b iF P Msg; move: (c3 (dst p) _ F)=>V;
        move/eqP: (HHold _ F)=>Eq; subst can_bc;
        rewrite (btExtend_seq_same V iB); by [|move: (HExt (dst p) _ F)].
     by move=>_ F'; move: (HHold _ F').
@@ -102,7 +131,7 @@ case: Iw=>_ [GStabW|GSyncW].
     case Msg: (msg p)=>[|||b|||]; rewrite Msg in P;
     do? by
     [NBlockMsg_dest_btChain q st p b Msg P H=>Hc; move: (HGt (dst p) bc' _ F Hc)].
-    by BlockMsg_dest q st b iF P Msg; move: (c3 (dst p) _ F)=>V;
+    by BlockMsg_dest q st (src p) b iF P Msg; move: (c3 (dst p) _ F)=>V;
        move/eqP=>Eq; subst bc';
        (have: (has_chain (btChain (blockTree st)) st)
           by rewrite/has_chain eqxx)=>O;
@@ -121,25 +150,50 @@ case: Iw=>_ [GStabW|GSyncW].
     * move/eqP=>Eq [Eq']; subst n' stPm;
       move=>z; specialize (H1 z); specialize (H2 z).
       rewrite H2 in H1; move=>H3. specialize (H1 H3).
-      case Msg: (msg p)=>[|n prs|pr||||]; rewrite Msg in P;
-      rewrite [procMsg _ _ _] surjective_pairing in P; case: P=><- _;
+      case Msg: (msg p)=>[|prs|||||]; rewrite Msg in P;
+      rewrite [procMsg _ _ _ _] surjective_pairing in P; case: P=><- _;
       destruct st; rewrite/procMsg/=; do? by [];
       do? rewrite /Protocol.peers in H1.
       by rewrite mem_undup mem_cat; apply/orP; left.
       by case: ifP=>_;
          [rewrite mem_undup|rewrite -cat1s mem_cat mem_undup; apply/orP; right].
-    * by move=>_ F'; clear H1; move: (HCliq n' _ F')=>H1;
+    * case: ifP=>//_.
+      by move=>_ F'; clear H1; move: (HCliq n' _ F')=>H1;
          move=>z; specialize (H1 z); specialize (H2 z);
          rewrite H2 in H1=>H3; specialize (H1 H3).
 
   (* applying conserved *)
   + move=>n' st'; rewrite findU c1 /=; case: ifP; last first.
-    * move=>NDst F'; move: (HExt _ st' F')=>->.
+    * move=>NDst F'; move: (HExt _ st' F').
       rewrite/blocksFor{2}/inFlightMsgs.
-      admit.
+      rewrite filter_cat map_cat foldl_cat.
+      have X: [seq msg_block (msg p0) | p0 <- seq.rem p (inFlightMsgs w) & dst p0 == n']
+              = [seq msg_block (msg p0) | p0 <- inFlightMsgs w & dst p0 == n'].
+      - elim : (inFlightMsgs w)=>//x xs Hi/=.
+        case:ifP=>[/eqP Z|_/=]; first by subst x; rewrite eq_sym NDst.
+        by case: ifP=>///eqP Z; subst n'; rewrite/= Hi.  
+      rewrite X; clear X=>E.
+      (* OK, now it's non-trivial, as we need to show that none of the
+         blocks in [seq msg_block (msg p0) | p0 <- ms & dst p0 == n']
+         affects the canonical block chain. This is even trickier, as
+         the block in the response might not be in the can_bc's
+         blocktree, yet it still doesn't affect the canonicity. Can we
+         derive it from canonicity, i.e. HGt? Perhaps, we need to
+         change the definition of largest_chain, so it would account
+         for _all_ the blocks. In other words, none of the blocks out
+         there can "spoil" the largest blockchain, should it be added
+         to its carrier block tree.
+
+         If this turns out to be too tricky, we can just prohibit, in
+         the invariant, to transmit connectivity-related messages.
+
+         I suggest to postpone this part of the proof for now to see
+         how others go, and then we decide how to change the invariant regarding the canonical          chain.  *)
+        admit.
+
     * move/eqP=>Eq [Eq']; subst n' stPm.
       case Msg: (msg p)=>[|||b|||]; rewrite Msg in P;
-      rewrite [procMsg _ _ _] surjective_pairing in P; case: P=>_ <-;
+      rewrite [procMsg _ _ _ _] surjective_pairing in P; case: P=>_ <-;
       rewrite/blocksFor/inFlightMsgs; simplw w=>_ ->; rewrite/procMsg.
-      destruct st=>/=; case: ifP.
-      move=>_.
+      destruct st=>/=. 
+      (* Move all non-interesting messages into a lemma *)
